theories/string_lang/StringLangProperties.v
@@ -6,11 +6,11 @@ Import ListNotations.
 
 
 Theorem compute_program_add : forall 
-  {k} (p_str : StringLang.program k) n n' snap, 
+  (p_str : StringLang.program) n n' snap, 
   StringLang.compute_program p_str snap (n + n') =
   StringLang.compute_program p_str (StringLang.compute_program p_str snap n') n.
 Proof.
-  intros k p_str. induction n; intros n' snap.
+  intros p_str. induction n; intros n' snap.
   - reflexivity.
   - simpl. rewrite IHn. reflexivity.
 Qed.
